PR feedback

DynamoDbEncryption/dafny/DynamoDbItemEncryptor/src/AwsCryptographyDynamoDbEncryptionItemEncryptorOperations.dfy
@@ -494,9 +494,9 @@ module AwsCryptographyDynamoDbEncryptionItemEncryptorOperations refines Abstract
   //= type=implication
   //# An item MUST be determined to be plaintext if it does not contain
   //# attributes with the names "aws_dbe_header" and "aws_dbe_footer".
-  function method IsPlaintextItem(ddbItem: ComAmazonawsDynamodbTypes.AttributeMap) : (ret: bool) {
-    !( && StructuredEncryptionUtil.HeaderField in ddbItem.Keys
-       && StructuredEncryptionUtil.FooterField in ddbItem.Keys)
+  predicate method IsPlaintextItem(ddbItem: ComAmazonawsDynamodbTypes.AttributeMap) {
+    && StructuredEncryptionUtil.HeaderField !in ddbItem.Keys
+    && StructuredEncryptionUtil.FooterField !in ddbItem.Keys
   }
 
   predicate EncryptItemEnsuresPublicly(input: EncryptItemInput, output: Result<EncryptItemOutput, Error>)
